Main.lean
@@ -13,34 +13,38 @@ namespace divseq2
   axiom h₀₇ (l : Nat) : 8 * l + 4 + (8 * l + 4 - 4) / 4 * 5 + 6 = (succ (l * 3)) * 2 * 3 + 2 + 2
   axiom h₀₈ (l : Nat) : 4 * (4 * l + 3) + (4 * l + 3 - 3) / 2 + 4 = (succ (succ (l * 3))) * 2 * 3 + 2 + 2
   axiom h₁₂ (l : Nat) : 9 * (2 * l) + 6 = (succ (l * 3 * 2)) * 3 + 1 + 2
+  axiom h₁₃ (l : Nat) : (9 * (4 * l + 1) + 15) / 2 = (succ (succ (l * 3) * 2)) * 3 + 1 + 2
+  axiom h₁₄ (l : Nat) : (9 * (8 * l + 7) + 9) / 4 = (succ (succ (succ (l * 3)) * 2)) * 3 + 1 + 2
   -- 十分条件
   theorem singleToExts (n : Nat) (p : SingleLimited (succ (succ n))) : ExtsLimited (n+2) := match p with
-    | SingleLimited.is02 l p2 => match p2 with
-      | ExtsLimited.is _ _ p3 _ _ _ _ _ _ _ _ _ => p3
+    | SingleLimited.is02 _ p2 => match p2 with
+      | ExtsLimited.is _ _ p3 _ _ _ _ _ _ _ _ _ _ _ => p3
     | SingleLimited.is03 m p2 => match p2 with
-      | ExtsLimited.is _ _ _ _ _ p3 _ _ _ _ _ _ => have p4 := Eq.subst (h₀₃ m) p3; p4
+      | ExtsLimited.is _ _ _ _ _ p3 _ _ _ _ _ _ _ _ => have p4 := Eq.subst (h₀₃ m) p3; p4
     | SingleLimited.is04 m p2 => match p2 with
-      | ExtsLimited.is _ _ _ _ _ _ _ _ _ _ p3 _ => have p4 := Eq.subst (h₀₄ m) p3; p4
+      | ExtsLimited.is _ _ _ _ _ _ _ _ _ _ p3 _ _ _ => have p4 := Eq.subst (h₀₄ m) p3; p4
     | SingleLimited.is05 m p2 => match p2 with
-      | ExtsLimited.is _ _ _ _ _ _ _ _ _ _ _ p3 => have p4 := Eq.subst (h₀₅ m) p3; p4
+      | ExtsLimited.is _ _ _ _ _ _ _ _ _ _ _ p3 _ _ => have p4 := Eq.subst (h₀₅ m) p3; p4
     | SingleLimited.is06 l p2 => match p2 with
-      | ExtsLimited.is _ _ _ _ _ _ _ p3 _ _ _ _ => have p4 := Eq.subst (h₀₆ l) p3; p4
+      | ExtsLimited.is _ _ _ _ _ _ _ p3 _ _ _ _ _ _ => have p4 := Eq.subst (h₀₆ l) p3; p4
     | SingleLimited.is07 l p2 => match p2 with
-      | ExtsLimited.is _ _ _ _ _ _ _ _ p3 _ _ _ => have p4 := Eq.subst (h₀₇ l) p3; p4
+      | ExtsLimited.is _ _ _ _ _ _ _ _ p3 _ _ _ _ _ => have p4 := Eq.subst (h₀₇ l) p3; p4
     | SingleLimited.is08 l p2 => match p2 with
-      | ExtsLimited.is _ _ _ _ _ _ _ _ _ p3 _ _ => have p4 := Eq.subst (h₀₈ l) p3; p4
-    | SingleLimited.is09 l p2 => match p2 with
-      | ExtsLimited.is _ _ _ p3 _ _ _ _ _ _ _ _ => p3
-    | SingleLimited.is11 k p2 => match p2 with
-      | ExtsLimited.is _ _ _ _ p3 _ _ _ _ _ _ _ => p3
+      | ExtsLimited.is _ _ _ _ _ _ _ _ _ p3 _ _ _ _ => have p4 := Eq.subst (h₀₈ l) p3; p4
+    | SingleLimited.is09 _ p2 => match p2 with
+      | ExtsLimited.is _ _ _ p3 _ _ _ _ _ _ _ _ _ _ => p3
+    | SingleLimited.is11 _ p2 => match p2 with
+      | ExtsLimited.is _ _ _ _ p3 _ _ _ _ _ _ _ _ _ => p3
     | SingleLimited.is12 l p2 => match p2 with
-      | ExtsLimited.is _ _ _ _ _ _ p3 _ _ _ _ _ => have p4 := Eq.subst (h₁₂ l) p3; p4
-    | SingleLimited.is13 l p2 => sorry
-    | SingleLimited.is14 l p2 => sorry
+      | ExtsLimited.is _ _ _ _ _ _ p3 _ _ _ _ _ _ _ => have p4 := Eq.subst (h₁₂ l) p3; p4
+    | SingleLimited.is13 l p2 => match p2 with
+      | ExtsLimited.is _ _ _ _ _ _ _ _ _ _ _ _ p3 _ => have p4 := Eq.subst (h₁₃ l) p3; p4
+    | SingleLimited.is14 l p2 => match p2 with
+      | ExtsLimited.is _ _ _ _ _ _ _ _ _ _ _ _ _ p3 => have p4 := Eq.subst (h₁₄ l) p3; p4
 
   axiom m₀₂₁ (l : Nat) : succ (succ (l - 2)) < succ (succ (succ (succ (succ (l * 2 * 2) * 3))))
-  axiom m₀₃₁ (m : Nat) : succ (succ (2 * (m - 1))) < succ (succ (succ (succ (succ (succ (m * 3 * 2) * 2) * 3))))
-  axiom m₀₃₂ (m : Nat) : 2 * (m - 1) + 2 = 2* m
+  axiom m₀₃₁ (m : Nat) : succ (succ (2 * m - 2)) < succ (succ (succ (succ (succ (succ (m * 3 * 2) * 2) * 3))))
+  axiom m₀₃₂ (m : Nat) : 2 * m - 2 + 2 = 2* m
   axiom m₀₄₁ (m : Nat) : succ (succ (4 * m + 1 - 2)) < succ (succ (succ (succ (succ (succ (succ (m * 3) * 2) * 2) * 3))))
   axiom m₀₄₂ (m : Nat) : 4 * m + 1 - 2 + 2 = 4 * m + 1
   axiom m₀₅₁ (m : Nat) : succ (succ (8 * m + 7 - 2)) < succ (succ (succ (succ (succ (succ (succ (succ (m * 3)) * 2) * 2) * 3))))
@@ -54,11 +58,15 @@ namespace divseq2
   axiom m₀₉₁ (j : Nat) : succ (succ (j - 2)) < succ (succ (j * 3))
   axiom m₀₉₂ (j : Nat) : j - 2 + 2 = j
   axiom m₁₁₁ (k : Nat) : succ (succ (k - 2)) < succ (succ (succ (k * 2 * 3)))
-  axiom m₁₂₁ (l : Nat) : succ (succ (2 * (l - 1))) < succ (succ (succ (succ (l * 3 * 2) * 3)))
+  axiom m₁₂₁ (l : Nat) : succ (succ (2 * l - 2)) < succ (succ (succ (succ (l * 3 * 2) * 3)))
+  axiom m₁₃₁ (l : Nat) : succ (succ (4 * l + 1 - 2)) < succ (succ (succ (succ (succ (l * 3) * 2) * 3)))
+  axiom m₁₃₂ (l : Nat) : 4 * l + 1 - 2 + 2 = 4 * l + 1
+  axiom m₁₄₁ (l : Nat) : succ (succ (8 * l + 7 - 2)) < succ (succ (succ (succ (succ (succ (l * 3)) * 2) * 3)))
+  axiom m₁₄₂ (l : Nat) : 8 * l + 7 - 2 + 2 = 8 * l + 7
   def makeLimitedDivSeq (x : Nat) (rs : ∀ x₁, x₁ < x → SingleLimited x₁) : SingleLimited x := match x with
     | 0             => SingleLimited.is10 -- 6*<0>+3 = 3
     | 1             => SingleLimited.is01 -- 6*<1>+3 = 9
-    | succ (succ x) => by cases (mod3 x) with
+    | succ (succ x) => by have rs := rs; cases (mod3 x) with
       -- 6 mod 9
       | threeZero j =>
           have sin := rs (succ (succ (j - 2))) (m₀₉₁ j); have ext := singleToExts (j - 2) sin; rw [m₀₉₂ j] at ext;
@@ -70,11 +78,17 @@ namespace divseq2
             exact SingleLimited.is11 k ext;
         | odd k  => cases (mod3 k) with
           | threeZero l =>
-              have sin := rs (succ (succ (2 * (l - 1)))) (m₁₂₁ l);
-              have ext := singleToExts (2 * (l - 1)) sin; rw [m₀₃₂ l] at ext;
+              have sin := rs (succ (succ (2 * l - 2))) (m₁₂₁ l);
+              have ext := singleToExts (2 * l - 2) sin; rw [m₀₃₂ l] at ext;
               exact SingleLimited.is12 l ext;
-          | threeOne l  => sorry
-          | threeTwo l  => sorry
+          | threeOne l  =>
+              have sin := rs (succ (succ (4 * l + 1 - 2))) (m₁₃₁ l);
+              have ext := singleToExts (4 * l + 1 - 2) sin; rw [m₁₃₂ l] at ext;
+              exact SingleLimited.is13 l ext;
+          | threeTwo l  =>
+              have sin := rs (succ (succ (8 * l + 7 - 2))) (m₁₄₁ l);
+              have ext := singleToExts (8 * l + 7 - 2) sin; rw [m₁₄₂ l] at ext;
+              exact SingleLimited.is14 l ext;
       -- 0 mod 9
       | threeTwo j  => cases (parity j) with
         | even k => cases (mod3 k) with
@@ -96,8 +110,8 @@ namespace divseq2
               exact SingleLimited.is02 l ext;
           | odd l  => cases (mod3 l) with
             | threeZero m =>
-                have sin := rs (succ (succ (2 * (m - 1)))) (m₀₃₁ m);
-                have ext := singleToExts (2 * (m - 1)) sin; rw [m₀₃₂ m] at ext;
+                have sin := rs (succ (succ (2 * m - 2))) (m₀₃₁ m);
+                have ext := singleToExts (2 * m - 2) sin; rw [m₀₃₂ m] at ext;
                 exact SingleLimited.is03 m ext;
             | threeOne m  =>
                 have sin := rs (succ (succ (4 * m + 1 - 2))) (m₀₄₁ m);
